maybe works

src/tactic/degeval.lean
@@ -7,16 +7,30 @@ namespace tactic.interactive
 setup_tactic_parser
 #check monoid.npow
 #check @has_pow.pow
-meta def monomial_weight (e : expr) : list expr :=
+
+
+example {n : ℕ} : 0 = n :=
+by do
+  `(%%tl = %%tr) ← target,
+  trace tl.to_nat
+--#exit
+--
+--  unify tl `(has_zero.zero.{0} nat nat.has_zero),
+--  let bo : bool := (tl = has_zero.zero nat nat.has_zero),
+--  trace tl.to_string
+
+
+/-
+meta def monomial_weight (e : expr) : expr :=
 match e.app_fn with
-| `(coe_fn $ polynomial.monomial %%n) := [n]
-| `(monoid.npow %%n %%x) := [n]
+| `(coe_fn $ polynomial.monomial %%n) := n
+| `(monoid.npow %%n %%x) := n
 | (app f a) := if f.get_app_fn.const_name = `has_pow.pow then
                         f.get_app_args else []
 --                        [a] else []
-| (app f a) := if f.get_app_fn.const_name = `polynomial.C then
-                  [] else
-                []
+--| (app f a) := if f.get_app_fn.const_name = `polynomial.C then
+--                  [] else
+--                []
 /-
                 if f.get_app_fn.const_name = `has_pow.pow then
                 match f.get_app_args with
@@ -29,6 +43,156 @@ match e.app_fn with
 -/
 | _ := []
 end
+-/
+#check list.erase
+#check expr.to_nat
+meta def guess_deg (e : expr) : tactic expr :=
+do n0 ← to_expr ``(nat.zero),
+   n1 ← to_expr ``(bit1 nat.zero),
+   pol ← to_expr ``(polynomial.X),pt ← infer_type pol, trace pt,
+match e.app_fn with
+--| (expr.app op a) := if (op.get_app_fn.const_name = `has_add.add) then a else a
+| `(coe_fn $ polynomial.monomial %%n) := return n
+| `(coe_fn $ polynomial.C) := --do `(some %%arg) ← e.get_app_args.nth 0, trace arg,
+                              return n0
+| a := do bo ← (succeeds $ unify e pol), if bo then return n1 else
+
+--let cond : bool := e = pol, trace cond,trace e, trace pol,
+       (--if cond then (do return n1) else
+            (do let margs := e.get_app_args,
+            hh ← margs.nth 4,
+            return hh) <|>
+            (do val ← to_expr ``(polynomial.nat_degree), return $ expr.mk_app val [e]))
+--| `(polynomial.C %%a) := return a
+--| a := do trace a, if a.const_name = ``polynomial.C then (do n0 ← to_expr ``(nat.zero), return n0) else
+--    (do val ← to_expr ``(polynomial.nat_degree), return $ expr.mk_app val [e])
+end
+
+meta def get_factors_add : expr → tactic expr
+| `(has_mul.mul %%a %%b) := do ga ← get_factors_add a, gb ← get_factors_add b,
+                              tot ← mk_app `has_add.add [ga, gb],
+                              return tot
+--| `(expr.app $ coe_fn $ polynomial.monomial %%n) := [n]
+| e := do ge ← guess_deg e, return ge
+
+
+meta def fina : tactic unit :=
+do `(polynomial.nat_degree %%tl = %%tr) ← target,
+  let summ := (get_summands tl),
+  let rere := summ.map get_factors_add,-- (get_factors_add t),
+  trace rere
+--  ret ← rere.foldl guess_deg t,
+
+
+end tactic.interactive
+
+open polynomial
+open_locale polynomial
+variables {R : Type*} [semiring R] {f g h : R[X]} {a b c d e : R}
+
+lemma pro {h : C d ≠ 0} :
+  nat_degree (monomial 5 c * monomial 1 c + f + monomial 7 d + C a * X ^ 0 + C b * X ^ 5 + C c * X ^ 2 + C d * X ^ 10 + C e * X + bit0 0 : R[X]) = 10 :=
+begin
+  fina,
+end
+
+
+meta def rec_ret_fac_add : expr → tactic (list (list expr))
+| e@`(%%_ + %%_)     := return_factors e
+| (expr.lam _ _ _ e) := rec_ret_fac e
+| (expr.pi  _ _ _ e) := rec_ret_fac e
+| e                  := do erf ← e.get_app_args.map rec_ret_fac,
+                          do ferf ← list.list_to_cat (erf),
+                          return ferf
+
+
+
+meta def get_factors : expr → tactic (list expr)
+| `(has_mul.mul %%a %%b) := do ga ← get_factors a, gb ← get_factors b, return (ga ++ gb)
+--| `(expr.app $ coe_fn $ polynomial.monomial %%n) := [n]
+| e := do ge ← guess_deg e, return [ge]
+
+meta def return_factors (e : expr) : tactic (list (list expr)) :=
+--let li_summands := get_summands e in
+do let ges := get_summands e in
+  do gls ← ges.mmap get_factors,
+  return gls
+
+def list.list_to_cat {α : Type*} : list (list α) → list α
+| [] := []
+| (l::ls) := l ++ ls.list_to_cat
+
+meta def rec_ret_fac : expr → tactic (list (list expr))
+| e@`(%%_ + %%_)     := return_factors e
+| (expr.lam _ _ _ e) := rec_ret_fac e
+| (expr.pi  _ _ _ e) := rec_ret_fac e
+| e                  := do erf ← e.get_app_args.map rec_ret_fac,
+                          do ferf ← list.list_to_cat (erf),
+                          return ferf
+
+meta def fina : tactic unit :=
+do t ← target,
+  let rere := (rec_ret_fac t),
+  ret ← rere.foldl guess_deg t,
+
+
+end tactic.interactive
+
+open polynomial
+open_locale polynomial
+variables {R : Type*} [semiring R] {f g h : R[X]} {a b c d e : R}
+
+lemma pro {h : C d ≠ 0} :
+  nat_degree (monomial 5 c * monomial 1 c + f + monomial 7 d + C a * X ^ 0 + C b * X ^ 5 + C c * X ^ 2 + C d * X ^ 10 + C e * X : R[X]) = 10 :=
+begin
+  fina,
+end
+
+
+/-
+meta def guess_deg : expr → tactic expr
+--match e.app_fn with
+--| (expr.app op a) := if (op.get_app_fn.const_name = `has_add.add) then a else a
+| `(coe_fn $ polynomial.monomial %%n) := return n
+--| `(polynomial.C %%a) := a
+| a := do val ← to_expr ``(polynomial.nat_degree), return $ expr.mk_app val [a]
+--end
+
+meta def to_oper (f₁ f₂ : name) : expr → tactic expr
+| (expr.app (expr.app op a) b) := do oa ← to_oper a, ob ← to_oper b,
+                                    if op.get_app_fn.const_name = f₁ then
+                                       (mk_app f₂ [oa, ob]) else (return (op oa ob))
+--  The rest of the match is unchanged
+| (expr.lam a b c e)         := do oc ← to_oper c, oe ← to_oper e,
+                                  return (expr.lam a b oc oe)
+| (expr.pi  a b c e)         := do oc ← to_oper c, oe ← to_oper e,
+                                  return (expr.pi  a b oc oe)
+| (expr.elet a b c e)        := do ob ← to_oper b, oc ← to_oper c, oe ← to_oper e,
+                                  return (expr.elet  a ob oc oe)
+| (expr.app a b)             := do oa ← to_oper a, ob ← to_oper b,
+                                  return (expr.app oa ob)
+| (expr.mvar u p e)          := do oe ← to_oper e,
+                                  return (expr.mvar u p oe)
+| (expr.local_const u p b e) := do oe ← to_oper e,
+                                  return (expr.local_const u p b oe)
+| (expr.macro md le)         := do ole ← le.mmap (to_oper),
+                                  return (expr.macro md ole)
+| e                          := return e
+
+
+
+meta def recurse_on_expr_ : expr → list expr
+| e@`(%%_ + %%_)     := get_summands e
+| (expr.app f a)     := let rho :=f.get_app_args.map get_summands in
+                          match rho with
+                          | [] := []
+                          | (r::rs) := r
+                          end
+--                          | _ := []
+--                        return $ list.foldl _ _ rho
+| (expr.lam _ _ _ e) := recurse_on_expr_ e
+| (expr.pi  _ _ _ e) := recurse_on_expr_ e
+| e                  := [e]
 
 /--  Assuming that the expression `e` consists of a product of `C a, monomial n b, X, X ^ d`,
 `get_exps` extracts the list of what should be the degrees of the factors. -/
@@ -53,6 +217,7 @@ meta def get_exps : expr → list expr
 -/
 --          end
 
+-/
 .
 #check coe_fn
 end tactic.interactive
@@ -64,20 +229,33 @@ variables {R : Type*} [semiring R] {f g h : R[X]} {a b c d e : R}
 lemma pro {h : C d ≠ 0} :
   nat_degree (monomial 5 c * monomial 1 c + f + monomial 7 d + C a * X ^ 0 + C b * X ^ 5 + C c * X ^ 2 + C d * X ^ 10 + C e * X : R[X]) = 10 :=
 by do t ← target,
-    --trace t,
+--    let rer := tactic.interactive.recurse_on_expr_ t,trace "rer",trace rer,trace "rer finito",trace t,
     match t.is_eq with
     | none := trace "target is not an equality"
     | some (tl, tr) := do
+--      trace tl,
       match tl with
       | (expr.app nd a) := if nd.get_app_fn.const_name = `polynomial.nat_degree then
           (let sus := (interactive.get_summands a) in
-          let ee : list (list expr) := list.map tactic.interactive.get_exps sus in
+            let fsu : list (list expr) := sus.map tactic.interactive.get_factors in
+            match fsu with
+            | [] := trace fsu
+            | (fff::fffs) := trace $ fff.map tactic.interactive.guess_deg
+--            let gd :=
+--            trace fsu
+--            else skip
+--            end
+--            sorry
+--#exit
+--          let ee : list (list expr) := list.map tactic.interactive.get_exps sus in
+/-
           match sus with
           | [] := skip
-          | (s1:: ss) := let vv := tactic.interactive.get_exps s1 in
-            trace ee
+          | (s1:: ss) := let vv := tactic.interactive.get_exps s1 in skip
+--            trace ee
             --trace format!"{s1.local_pp_name} and {vv}"
           end
+-/
 --          trace ee
           )
            else skip
